\newpage
\section{The Binomial Coefficient}

In this short section we will cover the definition and Properties of the binomial coefficient
without going to deep into the combinatorics meaning or Pascal's Triangle.

\[
    \binom{n}{k} := \frac{n!}{k!(n-k)!}
\]

or as Product 

\[
    \prod_{j = 1}^{n} \frac{n-k+j}{j},
\]

with \(n\) and \(k\) as natural numbers (for the moment).

\subsection{Properties}

\begin{itemize}
    
    \item \( \binom{n}{k} =  \binom{n}{n - k}\)
    
    \item \( \binom{n}{k - 1} = \binom{n}{k} \frac{n - k}{k + 1}\)
    
    \item \( \sum_{k = 0}^{n} \binom{n}{k} = 2^n\) 
    
    \item \( \sum_{k = 0}^{n} \binom{m}{k} = \binom{n + 1}{m + 1}\) 
    
    \item \(\binom{n}{0} = 1 = \binom{n}{n}\)
    
    \item \(\binom{n}{k}\ + \binom{n}{k + 1} = \binom{n + 1}{k + 1}\)
    
    \item \(\binom{n}{k} = {(-1)}^k \binom{k - n - 1}{k}\)

\end{itemize}

\subsection{The binomial Theorem}

\[
    (a + b)^n =\sum_{k = 0}^{n} \binom{n}{k}a^{n - k}b^k
\]


\textbf{Proof:}

We will prove that the inequality holds for any \(n\). 

For \(n\) we have \( (a + b)^n =\sum_{k = 0}^{n} \binom{n}{k}a^{n - k}b^k\)

For \(n + 1\) we get 

\[
    (a + b)^{n + 1} =\sum_{k = 0}^{n + 1} \binom{n + 1}{k}a^{n + 1 - k}b^k
\]

Now let us manipulate the expression to demonstrate our theorem.
Assume that the statement is true for some integer \(n \ge 0\), i.e.

\[
    (a+b)^n = \sum_{k=0}^n \binom{n}{k} a^{\,n-k} b^{\,k}.
\]

Now for some greater \(n\)

\[
    (a+b)^{n+1} = (a+b)(a+b)^n.
\]

Using the induction hypothesis,

\[
    (a+b)^{n+1} = (a+b) \sum_{k=0}^n \binom{n}{k} a^{\,n-k} b^{\,k}.
\]

Distribute:

\[
    (a+b)^{n+1} = \sum_{k=0}^n \binom{n}{k} a^{\,n+1-k} b^{\,k}
    + \sum_{k=0}^n \binom{n}{k} a^{\,n-k} b^{\,k+1}.
\]

In the second sum, change the index of summation by setting $j = k + 1$, then rename $j$ back to $k$:

\[
    \sum_{k=0}^n \binom{n}{k} a^{\,n-k} b^{\,k+1}
    = \sum_{k=1}^{n+1} \binom{n}{k-1} a^{\,n+1-k} b^{\,k}.
\]

Now combine both sums:

\[
    (a+b)^{n+1} = \sum_{k=0}^{n+1} 
    \left( \binom{n}{k} + \binom{n}{k-1} \right)
    a^{\,n+1-k} b^{\,k},
\]

where we use the convention \(\binom{n}{k} = 0$ for $k < 0$ or $k > n\).

By \emph{Pascalâ€™s Identity},

\[
    \binom{n}{k} + \binom{n}{k-1} = \binom{n+1}{k}.
\]

Therefore,

\[
    (a+b)^{n+1} = \sum_{k=0}^{n+1} \binom{n+1}{k} a^{\,n+1-k} b^{\,k}.
\]

\QED
