\newpage
\section{Trigonometry}

In this section, we will cover a variety of trigonometric functions and their properties.

\subsection{Trigonometric Functions}

\begin{itemize}

    \item \( \sin(x) = \frac{1}{\csc(x)} \)

    \item \( \cos(x) = \frac{1}{\sec(x)}\)

    \item \( \tan(x) = \frac{\sin(x)}{\cos(x)}\ = \frac{1}{\cot(x)}\)

    \item \( \csc(x) = \frac{1}{\sin(x)} \)

    \item \( \sec(x) = \frac{1}{\cos(x)} \)

    \item \( \cot(x) = \frac{\cos(x)}{\sin(x)} = \frac{1}{\tan(x)} \)

\end{itemize}

\subsection{SOH-CAH-TOA}

\begin{itemize}

    \item \( \sin(x) = \frac{\text{opposite}}{\text{hypotenuse}} \)

    \item \( \cos(x) = \frac{\text{adjacent}}{\text{hypotenuse}} \)

    \item \( \tan(x) = \frac{\text{opposite}}{\text{adjacent}} \)

\end{itemize}

\subsection{Pythagorean Identities}

\begin{itemize}

    \item \( \sin^2(x) + \cos^2(x) = 1 \)

    \item \( 1 + \tan^2(x) = \sec^2(x) \)

    \item \( 1 + \cot^2(x) = \csc^2(x) \)

\end{itemize}

\subsection{Sum and Difference Formulas}

\begin{itemize}

    \item \( \sin(a + b) = \sin(a)\cos(b) + \cos(a)\sin(b) \)

    \item \( \sin(a - b) = \sin(a)\cos(b) - \cos(a)\sin(b) \)

    \item \( \cos(a + b) = \cos(a)\cos(b) - \sin(a)\sin(b) \)

    \item \( \cos(a - b) = \cos(a)\cos(b) + \sin(a)\sin(b) \)

    \item \( \tan(a + b) = \frac{\tan(a) + \tan(b)}{1 - \tan(a)\tan(b)}\)

    \item \( \tan(a - b) = \frac{\tan(a) - \tan(b)}{1 + \tan(a)\tan(b)}\)
    
\end{itemize}

\begin{center}
\includegraphics{trig.jpg}
\end{center}

\subsection{Double Angle Formulas}

\begin{itemize}

    \item \( \sin(2x) = 2\sin(x)\cos(x) \)

    \item \( \cos(2x) = \cos^2(x) - \sin^2(x) = 2\cos^2(x) - 1 = 1 - 2\sin^2(x) \)

    \item \( \tan(2x) = \frac{2\tan(x)}{1 - \tan^2(x)}\)

    \item \( \csc(2x) = \frac{2\csc(x)\sec(x)}{1 - \tan^2(x)}\)

    \item \( \sec(2x) = \frac{1 + \tan^2(x)}{2\tan(x)}\)

    \item \( \cot(2x) = \frac{1 - \tan^2(x)}{2\tan(x)}\)

\end{itemize}

\subsection{Half Angle Formulas}

\begin{itemize}

    \item \( \sin\left(\frac{x}{2}\right) = \pm\sqrt{\frac{1 - \cos(x)}{2}} \)

    \item \( \cos\left(\frac{x}{2}\right) = \pm\sqrt{\frac{1 + \cos(x)}{2}} \)

    \item \( \tan\left(\frac{x}{2}\right) = \frac{\sin(x)}{1 + \cos(x)} = \frac{1 - \cos(x)}{\sin(x)} = 
          \frac{\tan(x)}{1 + \tan^2(x)}\)

    \item \( \csc\left(\frac{x}{2}\right) = \frac{1}{\sin\left(\frac{x}{2}\right)} = 
          \pm\sqrt{\frac{2}{1 - \cos(x)}} \)

    \item \( \sec\left(\frac{x}{2}\right) = \frac{1}{\cos\left(\frac{x}{2}\right)} = 
          \pm\sqrt{\frac{2}{1 + \cos(x)}} \)

    \item \( \cot\left(\frac{x}{2}\right) = \frac{1}{\tan\left(\frac{x}{2}\right)} = 
          \frac{1 + \cos(x)}{\sin(x)} = \frac{1 - \tan^2(x)}{2\tan(x)}\)

\end{itemize}

\subsection{Product to Sum Formulas}

\begin{itemize}

    \item \( \sin(a)\sin(b) = \frac{1}{2}[\cos(a - b) - \cos(a + b)] \)

    \item \( \cos(a)\cos(b) = \frac{1}{2}[\cos(a - b) + \cos(a + b)] \)

    \item \( \sin(a)\cos(b) = \frac{1}{2}[\sin(a + b) + \sin(a - b)] \)

    \item \( \cos(a)\sin(b) = \frac{1}{2}[\sin(a + b) - \sin(a - b)] \)

\end{itemize}

\subsection{Power Reducing Formulas}

\begin{itemize}

    \item \( \sin^2(x) = \frac{1 - \cos(2x)}{2} \)

    \item \( \cos^2(x) = \frac{1 + \cos(2x)}{2} \)

    \item \( \tan^2(x) = \frac{1 - \cos(2x)}{1 + \cos(2x)}\)

    \item \( \csc^2(x) = \frac{1}{\sin^2(x)} = \frac{2}{1 - \cos(2x)} \)

    \item \( \sec^2(x) = \frac{1}{\cos^2(x)} = \frac{2}{1 + \cos(2x)} \)

    \item \( \cot^2(x) = \frac{1}{\tan^2(x)} = \frac{1 + \cos(2x)}{1 - \cos(2x)}\)

\end{itemize}

\subsection{Even and Odd Functions}

\begin{itemize}

    \item \( \sin(-x) = -\sin(x) \)

    \item \( \cos(-x) = \cos(x) \)

    \item \( \tan(-x) = -\tan(x) \)

    \item \( \csc(-x) = -\csc(x) \)

    \item \( \sec(-x) = \sec(x) \)

    \item \( \cot(-x) = -\cot(x) \)

\end{itemize}

\subsection{Graph Identity}

\(\cos(x) = \sin(x + \frac{\pi}{2})\)

\subsection{Trigonometric Values}
\smallskip

\begin{center}
    \renewcommand{\arraystretch}{1.4}
    \begin{tabular}{|c|c|c|c|}
    \hline
    \(\theta\) (radians) & \(\sin(\theta)\) & \(\cos(\theta)\) & \(\tan(\theta)\) \\
    \hline
    \(0\) & \(0\) & \(1\) & \(0\) \\
    \hline
    \(\frac{\pi}{6}\) & \(\frac{1}{2}\) & \(\frac{\sqrt{3}}{2}\) & \(\frac{1}{\sqrt{3}}\) \\
    \hline
    \(\frac{\pi}{4}\) & \(\frac{\sqrt{2}}{2}\) & \(\frac{\sqrt{2}}{2}\) & \(1\) \\
    \hline
    \(\frac{\pi}{3}\) & \(\frac{\sqrt{3}}{2}\) & \(\frac{1}{2}\) & \(\sqrt{3}\) \\
    \hline
    \(\frac{\pi}{2}\) & \(1\) & \(0\) & undefined \\
    \hline
    \(\frac{2\pi}{3}\) & \(\frac{\sqrt{3}}{2}\) & \(-\frac{1}{2}\) & \(-\sqrt{3}\) \\
    \hline
    \(\frac{3\pi}{4}\) & \(\frac{\sqrt{2}}{2}\) & \(-\frac{\sqrt{2}}{2}\) & \(-1\) \\
    \hline
    \(\frac{5\pi}{6}\) & \(\frac{1}{2}\) & \(-\frac{\sqrt{3}}{2}\) & \(-\frac{1}{\sqrt{3}}\) \\
    \hline
    \(\pi\) & \(0\) & \(-1\) & \(0\) \\
    \hline
    \(\frac{7\pi}{6}\) & \(-\frac{1}{2}\) & \(-\frac{\sqrt{3}}{2}\) & \(\frac{1}{\sqrt{3}}\) \\
    \hline
    \(\frac{5\pi}{4}\) & \(-\frac{\sqrt{2}}{2}\) & \(-\frac{\sqrt{2}}{2}\) & \(1\) \\
    \hline
    \(\frac{4\pi}{3}\) & \(-\frac{\sqrt{3}}{2}\) & \(-\frac{1}{2}\) & \(\sqrt{3}\) \\
    \hline
    \(\frac{3\pi}{2}\) & \(-1\) & \(0\) & undefined \\
    \hline
    \(\frac{5\pi}{3}\) & \(-\frac{\sqrt{3}}{2}\) & \(\frac{1}{2}\) & \(-\sqrt{3}\) \\
    \hline
    \(\frac{7\pi}{4}\) & \(-\frac{\sqrt{2}}{2}\) & \(\frac{\sqrt{2}}{2}\) & \(-1\) \\
    \hline
    \(\frac{11\pi}{6}\) & \(-\frac{1}{2}\) & \(\frac{\sqrt{3}}{2}\) & \(-\frac{1}{\sqrt{3}}\) \\
    \hline
    \(2\pi\) & \(0\) & \(1\) & \(0\) \\
    \hline
    \end{tabular}
\end{center}

\subsection{Unit Circle and Trigonometric Functions}

The unit circle is a circle with a radius of 1 centered at the origin. Trigonometric functions like 
\(\sin(\theta)\), \(\cos(\theta)\), and \(\tan(\theta)\) can be defined based on the coordinates of a 
point on the circle corresponding to angle \(\theta\).

\begin{center}
\begin{tikzpicture}[scale=3]
    % Draw unit circle
    \draw[thick] (0,0) circle (1);
    
    % Axes
    \draw[->] (-1.2,0) -- (1.2,0) node[right] {\(x\)};
    \draw[->] (0,-1.2) -- (0,1.2) node[above] {\(y\)};
    
    % Angle and triangle
    \draw[thick, blue] (0,0) -- ({cos(45)},{sin(45)}) node[pos=0.5, above left] {\(r=1\)};
    \draw[thick, red] (0,0) -- ({cos(45)},0);
    \draw[thick, green!60!black] ({cos(45)},0) -- ({cos(45)},{sin(45)});
    
    % Dotted lines
    \draw[dashed] ({cos(45)},{sin(45)}) -- ({cos(45)},0);
    
    % Angle arc
    \draw[->] (0.5,0) arc[start angle=0,end angle=45,radius=0.5];
    \node at (0.6,0.1) {\(\theta\)};
    
    % Labels
    \node[below right] at ({cos(45)},0) {\(\cos(\theta)\)};
    \node[left] at ({cos(45)},{sin(45)}) {\(\sin(\theta)\)};
    \node[right] at ({cos(45)}, {sin(45)/2}) {\(\tan(\theta)\)};
\end{tikzpicture}
\end{center}

\subsection{Definitions on the Unit Circle:}

\begin{itemize}

    \item \(\cos(\theta)\) is the \emph{x-coordinate} of the point on the circle.

    \item \(\sin(\theta)\) is the \emph{y-coordinate}.

    \item \(\tan(\theta) = \dfrac{\sin(\theta)}{\cos(\theta)}\) is the ratio of the opposite side to 
          the adjacent side in the triangle.

\end{itemize}

\subsection{Trigonometric Rules}

\begin{itemize}

    \item \(\frac{\sin \alpha}{a} = \frac{\sin \beta}{b} = \frac{\sin \gamma}{c}\)

    \item \(c^2 = a^2 + b^2 - 2ab \cos \gamma\)

    \item \(\frac{a - b}{a + b} = \frac{\tan \frac{1}{2}(\alpha - \beta)}{\tan \frac{1}{2} (\alpha + \beta)}\)

\end{itemize}

\subsection{Proof of the Cosine Rule}

The \emph{Cosine Rule} relates the lengths of the sides of a triangle to the cosine of one of its angles. 
For any triangle \( ABC \) with sides \( a = BC \), \( b = AC \), and \( c = AB \), and angle 
\( \gamma = \angle ACB \), the cosine rule states:

\[
    c^2 = a^2 + b^2 - 2ab\cos(\gamma)
\]

\textbf{Proof:}

Consider triangle \( ABC \), and place it on the coordinate plane such that point \(c\) is at the origin
\( (0,0) \), point \(B\) is at \( (a,0) \), and point \(A\) lies somewhere in the plane. 
Let angle \( \gamma = \angle ACB \).

Let the coordinates of point \(A\) be \( (b\cos\gamma, b\sin\gamma) \), since \( b = AC \) and weâ€™re 
using polar coordinates to define its location relative to point \(c\).

Using the distance formula to find side \( c = AB \), we get:

\begin{align*}
    c^2 &= {(a - b\cos\gamma)}^2 + {(0 - b\sin\gamma)}^2 \\
    &= a^2 - 2ab\cos\gamma + b^2\cos^2\gamma + b^2\sin^2\gamma \\
    &= a^2 + b^2(\cos^2\gamma + \sin^2\gamma) - 2ab\cos\gamma \\
    &= a^2 + b^2 - 2ab\cos\gamma
\end{align*}

Since \( \cos^2\gamma + \sin^2\gamma = 1 \).

Thus, we have proven that:

\[
    c^2 = a^2 + b^2 - 2ab\cos\gamma
\]

\QED
