\newpage
\section{The Natural Numbers}

In this section we will take a look at the natural numbers, which are the numbers we use for counting. 
The natural numbers are defined as follows:

We will now define the set of natural numbers, \( \Naturals \), via the following 9 axioms. 
These axioms are known as the \emph{Peano Axioms}. The first 4 axioms define equality on 
the set \( \Naturals \).

\begin{enumerate}[label=\Roman*.]

	\item For every \( x \in \Naturals \), we have \( x = x \).\hfill (Reflexivity)
	
	\item For every \( x, y \in \Naturals \), if \( x = y \) then \( y = x \).\hfill (Symmetry)
	
	\item For every \( x, y, z \in \Naturals \), if \( x = y \) and \( y = z \) then \( x = z \).\hfill 
	      (Transitivity)
	
	\item For all \( x, y \), if \( x \in \Naturals \) and \( x = y \), then \( y \in \Naturals \).\hfill 
	      (Closure of Equality)

\end{enumerate}

The remaining 5 axioms define the structure of \( \Naturals \):

\begin{enumerate}[label=\Roman*.]
	\setcounter{enumi}{4}

	\item \( 1 \in \Naturals \)
	
	\item If \( x \in \Naturals \), then the successor \( S(x) \in \Naturals \).
	
	\item There is no \( x \in \Naturals \) such that \( S(x) = 1 \).
	
	\item For all \( x, y \in \Naturals \), if \( S(x) = S(y) \), then \( x = y \).
	
	\item Let \( P(x) \) be a statement about the natural number \(x\). If:
	
		\begin{itemize}
	
			\item \( P(1) \) is true, and
	
			\item for all \( n \in \Naturals \), if \( P(n) \) is true, then \( P(S(n)) \) is also true,
	
		\end{itemize}
	
		then \( P(x) \) is true for all \( x \in \Naturals \).\hfill (Mathematical Induction)
\end{enumerate}

As shorthand, we denote:

\[
	S(1) = 2, \quad S(S(1)) = 3, \quad S(S(S(1))) = 4, \quad \text{and so on.}
\]

\subsection{Propositions and Proofs}

\subsubsection{Proposition 1: \texorpdfstring{\(n \ne m \implies S(n) \ne S(m)\)}{n!= m implies S (n)!=S (m)}}

\textbf{Proof:} 

We will prove this by contradiction. Assume \( n \ne m \) and \( S(n) = S(m) \). 
By Axiom 8, we have \( n = m \), which is a contradiction. Therefore, \( S(n) \ne S(m) \).

\subsubsection{Proposition 2: \texorpdfstring{\text{For any} \(n \in \Naturals,\ n \ne S(n)\)}{ For any n in N, n!= S (n)}}

\textbf{Proof:} 

\(M = \{n \in \Naturals \| n \ne S(n) \}\ \)

By \(1 \ne S(n)\ \) for any \(n \in \Naturals\), this implies that 1 is part of the set \(M\). 
This implies that \(S(n) \ne S(S(n)) \implies S(n) \in M\ \) By Axiom 9 \(M = \Naturals\)

\subsubsection{Proposition 3: \texorpdfstring{\(n \ne 1\ \exists m \in \Naturals \mid n = S(m)\)}{n!= 1, exists m in N | n = S (m)}}

\textbf{Proof:}

\[
	M = \{1\} \cup\{n \in \Naturals | \text{Proposition 3 is true}\}
\]

We know that 1 ins in the set \(M\). And by proposition 1 we know that

\[
	S(n) = S(S(m)) \implies S(n) \in M
\]

And by Axiom 9 we know that \(M = \Naturals\)

\subsection{Definition of Addition in \texorpdfstring{\(\Naturals\)}{}}

For any pair n, m \(\in \Naturals\) there is a unique way to define

\[
	\text{Add}(n , m) = n + m
\]

\begin{enumerate}
	
	\item \textbf{Base Case:} \(n + 1 = S(n)\)

	\item \textbf{Inductive Step:} \(n + S(m) = S(n + m) \iff S(n + m)\)

\end{enumerate}

\textbf{Uniqueness:} 

Suppose: \textit{A} \& \textit{B} satisfy our conditions. Fix n and then let \(M = \{ m \in \Naturals | 
A(n,m) = B(n, m)\}\). Then

\[
	A(n,1) = S(n) = B(n,1) \implies 1 \in M
\]

\[
	m \in M \implies A(n, m) = B(n, m) \implies A(n, S(m)) = S(A(n, m)) = S(B(n, m)) = B(n, S(m))
\]

\[
	\implies A(n , S(m)) = B(n, S(m))
\]

by Axiom 9 we know that \(M = \Naturals\) and A = B

\textbf{Construction:} For \(n = 1\) Define \(A(n, m) = S(m)\)

\begin{enumerate}
	
	\item \(A(n, 1) = S(n) = S(1)\)
	
	\item \(A(n, S(m)) = S(A(n, m)) = S(S(m))\)

\end{enumerate}

Define: \(A(S(n), S(m)) = S(A(n, m))\)

\begin{enumerate}

	\item \(A(S(n), 1) = S(A(n, 1)) = S(S(n))\)

	\item \(A(S(n), S(m)) = S(A(n, m)) = S(S(m))\)

\end{enumerate}

\textbf{Commutativity of Addition:}

The proposition says \(n + m = m + n\) for any \(n, m \in \Naturals\). We will prove this by 
induction on \(m\). Fix n and consider \(M = \{ n \in \Naturals | A(n, m) = A(n, m)\}\)

Now recall that \(A(n, 1) = S(n)\)

For \(n = 1\):

\[
	A(n, 1) = S(1) = A(1, n) \implies 1 \in \Naturals
\]

also \(A(n , k) = 1 + k \implies 1 + m = S(m) \implies 1 + m = m + 1 \implies 1 \in \Naturals\)

Suppose: \(n \in \Naturals \implies n + m = m + n\) or \(A(n, m) = A(m, n)\)

By construction \(A(S(n), m) = S(A(n, m))\) and by definition
\(A(S(n), m) = S(A(n, m)) = A(m, S(n)) = S(n) + m =  m + S(n) \implies S(n) \in M \implies 
\text{by induction } M = \Naturals\).
